Protocol/SAMLProtocol.fst
@@ -1,19 +1,22 @@
 module SamlProtocol
 
+open Crypto
 (*open Network*)
 
 type assertiontoken = string (*Add refinements*)
 type signedtoken = string (*Add refinements*)
 type id = string
 type endpoint = string
+type uri = string
 
 type Assertion =
-  | UnsignedAssertion: assertiontoken -> Assertion
+  | SignedAssertion: assertiontoken -> dsig -> Assertion
+  | EncryptedAssertion: encrypter:prin -> prinencryptedtoken:string -> Assertion
 
 type SamlMessage =
   | Login: uri -> SamlMessage
-  | AuthnRequest: issuer:prin -> id -> destination:endpoint -> dsig -> SamlMessage
-  | ResponseMessage: issuer:prin -> id -> inresto:id -> destination:endpoint -> Assertion -> SamlMessage
+  | AuthnRequest: issuer:prin ->  destination:endpoint -> message:string -> dsig -> SamlMessage
+  | AuthResponseMessage: issuer:prin -> destination:endpoint -> Assertion -> SamlMessage
   | LoginResponse: string -> SamlMessage
   | Failed: int -> SamlMessage
 
@@ -22,12 +25,10 @@ type SamlStatus =
   | Requester: SamlStatus
   | Responder: SamlStatus
 
-(*Verification*)
-type Log :: prin => samlmessage => E
-type Log2 :: string => string => nonce => E
 
 val SendSaml: prin -> SamlMessage -> unit
 val RecieveSaml: prin -> SamlMessage 
 
 val IssuerAssertion: issuer:prin -> subject:prin -> audience:prin -> inresto:id -> assertiontoken
 val AddSignatureToAssertion: assertiontoken -> dsig -> signedtoken
+val CreateAuthnRequestMessage: issuer:prin -> destination:prin -> string
