Protocol/xserver.fst
@@ -1,17 +1,41 @@
 module Serviceprovider
 
-open Lib
-open SessionManager
-open ContentServer
-open Protocol
-open Saml
+open SamlProtocol
 open Crypto
-open Network
+
+
 
 val serviceprovider:  me:prin -> pubkey me -> privkey me ->
-                      browser:prin -> idp:prin -> pubkey idp -> unit 
-let serviceprovider me pubk privk browser idp pubkidp = 
-  let req = Recieve browser in (*1*) (*7*)
+                      client:prin -> idp:prin -> pubkey idp -> unit 
+let serviceprovider me pubk privk client idp pubkidp = 
+ let req = RecieveSaml client in
+ match req with
+  | Login (url) -> (*Create AuthnRequest and send back*)
+    let authnReq = CreateAuthnRequestMessage me idp in
+    assume(Log me authnReq) (*Protocol event*);
+    let sigSP = Sign me privk authnReq in
+    let resp = AuthnRequest me idp authnReq sigSP in 
+    SendSaml client resp; (*2*)
+    serviceprovider me pubk privk client idp pubkidp (*Start over*)
+
+  | AuthResponseMessage (issuer, destination, assertion) -> 
+    match assertion with
+    | SignedAssertion (token,sigIDP) ->
+      if VerifySignature idp pubkidp token sigIDP
+      then
+        (assert(Log idp token);
+        let resp = LoginResponse "You are now logged in" in
+        SendSaml client resp) (*8*)
+      else SendSaml client (Failed 403);(*8.1*)
+      serviceprovider me pubk privk client idp pubkidp (*Start over*)
+  | _ -> SendSaml client (Failed 400);(*8.1*)
+        serviceprovider me pubk privk client idp pubkidp (*Start over*)
+
+
+
+
+
+(*  let req = Recieve client in (*1*) (*7*)
   match req with
   | Get (uri,params,cookies) -> 
 
@@ -38,3 +62,4 @@ let serviceprovider me pubk privk browser idp pubkidp =
       else Send (ErrorResponse 403 (getErrorPage 403) [])(*8.1*)
   
   | _ -> Send (ErrorResponse 400 (getErrorPage 400) [])
+*)
